# Question 

Sometimes it's possible to use induction backwards, proving things from $n$ to $n − 1$ instead of vice versa! For example, consider the statement $P(n)$ :
$x_1 ... x_n \le (\frac{x_1 + ... + x_n}{n})^n$, if $x_1, ... , x_n \ge 0$.

This is true when $n = 2$, since $(x_1 + x_2)^2 − 4x_1x_2 = (x1 − x2)^2 \ge 0$. 

### a By setting $x_n = \frac{x_1 + ... + x_{n−1}}{n − 1}$, prove that $P(n)$ implies $P(n − 1)$ whenever $n \gt 1$.
### b Show that $P(n)$ and $P(2)$ imply $P(2n)$. 
### c Explain why this implies the truth of $P(n)$ for all $n$.

# Answer

### a

$x_1 ... x_n \le (\frac{x_1 + ... + x_n}{n})^n$, if $x_1, ... , x_n \ge 0$.
$x_1 ... x_{n-1}\frac{x_1 + ... + x_{n−1}}{n − 1} \le (\frac{x_1 + ... + x_{n-1}+\frac{x_1 + ... + x_{n−1}}{n − 1}}{n})^n$
$x_1 ... x_{n-1}\frac{x_1 + ... + x_{n−1}}{n − 1} \le (\frac{\frac{n}{n-1}(x_1 + ... + x_{n-1})}{n})^n=(\frac{x_1+...+x_{n-1}}{n-1})^n$
$x_1 ... x_{n-1} \le (\frac{x_1+...+x_{n-1}}{n-1})^{n-1}$

QED.

### b

$x_1 ... x_n \le (\frac{x_1 + ... + x_n}{n})^n$, if $x_1, ... , x_n \ge 0$.
$x_1x_2\le(\frac{x_1+x_2}{2})^2$
let $x_n = {x_n}_1{x_n}_2$
$x_1 ... x_n = {x_1}_1{x_1}_2...{x_n}_1{x_n}_2\le(\frac{{x_1}_1+{x_1}_2}{2})(\frac{{x_1}_1+{x_1}_2}{2})...(\frac{{x_n}_1+{x_n}_2}{2})(\frac{{x_n}_1+{x_n}_2}{2})\le(\frac{\frac{{x_1}_1+{x_1}_2}{2}+\frac{{x_1}_1+{x_1}_2}{2}...+\frac{{x_n}_1+{x_n}_2}{2}+\frac{{x_n}_1+{x_n}_2}{2}}{2n})^{2n}$

QED.

### c

$\forall{x} < n$ ,use conclusion a.
$\forall{x} > n$ , there always $\exists{n_0}$, make $n_0 \le x \le 2n_0 $ ,use conclusion a and conclusion b.